\documentclass{article}
\usepackage{epsfig}
% Packages requested by user
\usepackage{amsmath}

\pagestyle{empty}
\begin{document}
$ \rho = \rho_0 e^{-h/H} $
\pagebreak

$ \rho_0 $
\pagebreak

$ h $
\pagebreak

$ H $
\pagebreak

$ p = \rho RT $
\pagebreak

\begin{eqnarray*} x( t ) = \frac{ \dot{ x }_0 }{ n } \sin( n t ) - \left( 3 x_0 + \frac{ 2 \dot{ y }_0 } { n } \right) \cos( n t ) + \left( 4 x_0 + \frac{ 2 \dot{ y }_0 }{ n } \right) \\ y( t ) = \left( 6 x_0 + \frac{ 4 \dot{ y_0 } }{ n } \right) \sin( n t ) + \frac{ 2 \dot{ x }_0 }{ n } \cos( n t ) - ( 6 x_0 n + 3 \dot{ y_0 } ) t + \left( y_0 - \frac{ 2 \dot{ x }_0 }{ n } \right) \\ z( t ) = \frac{ \dot{ z }_0 }{ n } \sin( n t ) + z_0 \cos ( n t ) \\ \dot{ x }( t ) = ( 3 x_0 n + 2 \dot{ y }_0 ) \sin( n t ) + \dot{ x }_0 \cos( n t ) \\ \dot{ y }( t ) = - 2 \dot{ x }_0 \sin( n t ) + ( 6 x_0 n + 4 \dot{ y }_0 ) \cos( n t) - ( 6 n x_0 + 3 \dot{ y }_0 ) \\ \dot{ z }( t ) = - z_0 n \sin( n t ) + \dot{ z }_0 \cos( n t ) \end{eqnarray*}
\pagebreak

$ x( t ) $
\pagebreak

$ y( t ) $
\pagebreak

$ z( t ) $
\pagebreak

$ x_0 $
\pagebreak

$ y_0 $
\pagebreak

$ z_0 $
\pagebreak

$ n $
\pagebreak

$ t $
\pagebreak

\[ f( E ) = E - e * sin( E ) - M \]
\pagebreak

$ E $
\pagebreak

$ e $
\pagebreak

$ M $
\pagebreak

\[ \frac{ df( E ) } { dE } = 1 - e * cos( E ) \]
\pagebreak

\[ f( F ) = e * sinh( F ) - F - M \]
\pagebreak

$ F $
\pagebreak

\[ \frac{ df( F ) } { dF } = e * cosh( F ) - 1 \]
\pagebreak

\[ \bar{f} = q * \bar{v} x \bar{B} \]
\pagebreak

$f$
\pagebreak

$q$
\pagebreak

$\bar{v}$
\pagebreak

$\bar{B}$
\pagebreak

\[ \bar{a}_{gravity} = -\frac{G * m_{2}}{r_{12}^{3}} * \bar{r}_{12} \]
\pagebreak

$G$
\pagebreak

$m_{2}$
\pagebreak

$\bar{r}_{12}$
\pagebreak

\[ \bar{a}_{gravity} = -\frac{\mu_{2}}{r_{12}^{3}} * \bar{r}_{12} \]
\pagebreak

$\mu_{2}$
\pagebreak

\[ \bar{F}_{gravity} = -\frac{G * m_{1} * m_{2}}{r_{12}^{3}} * \bar{r}_{12} \]
\pagebreak

$m_{1}$
\pagebreak

\[ \bar{F}_{gravity} = -\frac{m_{1} * \mu_{2}}{r_{12}^{3}} * \bar{r}_{12} \]
\pagebreak

\begin{eqnarray*} {a}_{gravity,x} &=& -\mu_{2}*\frac{x_{1}-x_{2}}{r^{3}} * \frac{3}{2}*J_{2} * \left(\frac{R}{r}\right)^{2} * (1-5*\hat{z}^2) \\ {a}_{gravity,y} &=& -\mu_{2}*\frac{y_{1}-y_{2}}{r^{3}} * \frac{3}{2}*J_{2} * \left(\frac{R}{r}\right)^{2} * (1-5*\hat{z}^2) \\ {a}_{gravity,z} &=& \frac{-\mu_{2}}{r^{2}} * \frac{3}{2}*J_{2} * \left(\frac{R}{r}\right)^{2} * (3-5*\hat{z}^2) * \hat{z} \\ \end{eqnarray*}
\pagebreak

$\hat{z} = \frac{z}{r}$
\pagebreak

$x$
\pagebreak

$y$
\pagebreak

$z$
\pagebreak

$r$
\pagebreak

$J_{2}$
\pagebreak

\begin{eqnarray*} {a}_{gravity,x} &=& -\mu_{2}*\frac{x_{1}-x_{2}}{r^{3}} * \frac{5}{2}*J_{3} * \left(\frac{R}{r}\right)^{3} * (3-7*\hat{z}^2) * \hat{z} \\ {a}_{gravity,y} &=& -\mu_{2}*\frac{y_{1}-y_{2}}{r^{3}} * \frac{5}{2}*J_{3} * \left(\frac{R}{r}\right)^{3} * (3-7*\hat{z}^2) * \hat{z} \\ {a}_{gravity,z} &=& \frac{-\mu_{2}}{r^{2}} * \frac{5}{2}*J_{3} * \left(\frac{R}{r}\right)^{3} * (-\frac{3}{5}+6*\hat{z}^2-7*\hat{z}^4) \\ \end{eqnarray*}
\pagebreak

$J_{3}$
\pagebreak

\begin{eqnarray*} {a}_{gravity,x} &=& \mu_{2}*\frac{x_{1}-x_{2}}{r^{3}} * \frac{35}{8}*J_{4} * \left(\frac{R}{r}\right)^{4} * (\frac{3}{7}-6*\hat{z}^2+9*\hat{z}^{4}) \\ {a}_{gravity,y} &=& \mu_{2}*\frac{y_{1}-y_{2}}{r^{3}} * \frac{35}{8}*J_{4} * \left(\frac{R}{r}\right)^{4} * (\frac{3}{7}-6*\hat{z}^2+9*\hat{z}^{4}) \\ {a}_{gravity,z} &=& \frac{\mu_{2}}{r^{2}} * \frac{35}{8}*J_{4} * \left(\frac{R}{r}\right)^{4} * (\frac{15}{7}-10*\hat{z}^2+9*\hat{z}^4) * \hat{z} \\ \end{eqnarray*}
\pagebreak

$J_{4}$
\pagebreak

$n$
\pagebreak

\begin{eqnarray*} {a}_{gravity sum,x} &=& {a}_{gravity central,x} + \sum\limits_{i=2}^{n} {a}_{gravity J_{n},x} \\ {a}_{gravity sum,y} &=& {a}_{gravity central,y} + \sum\limits_{i=2}^{n} {a}_{gravity J_{n},y} \\ {a}_{gravity sum,z} &=& {a}_{gravity central,z} + \sum\limits_{i=2}^{n} {a}_{gravity J_{n},z} \\ \end{eqnarray*}
\pagebreak

$J_{n}$
\pagebreak

\[ C_{J} = x^{2} + y^{2} + 2 * \left(\frac{1-\mu}{r_{1}} + \frac{\mu}{r_{2}}\right) - V^{2}, \]
\pagebreak

$C_{J}$
\pagebreak

$mu$
\pagebreak

$r_{1}$
\pagebreak

$r_{2}$
\pagebreak

$V$
\pagebreak

\begin{eqnarray*} \bar{ C }_{ n, m } = \Pi_{ n, m } C_{ n, m } \\ \bar{ S }_{ n, m } = \Pi_{ n, m } S_{ n, m } \end{eqnarray*}
\pagebreak

$ \bar{ C }_{ n, m } $
\pagebreak

$ \bar{ S }_{ n, m } $
\pagebreak

$ m $
\pagebreak

$ C_{ n, m } $
\pagebreak

$ S_{ n, m } $
\pagebreak

$ \Pi_{ n, m } $
\pagebreak

\[ \Pi_{ n, m } = \sqrt{ \frac{ ( n + m )! }{ ( 2 - \delta_{ 0, m } ) ( 2 n + 1 ) ( n - m )! } } \]
\pagebreak

$ \delta_{ 0, m } $
\pagebreak

$ \theta $
\pagebreak

\[ r ( \theta ) = \frac{ 1 } { a + b \cos( \theta + c ) + d \theta^3 + e \theta^4 + f \theta^5 + g \theta^6 } \]
\pagebreak

$ r $
\pagebreak

$ ( a, b, c, d, e, f, g ) $
\pagebreak

$ d $
\pagebreak

\[ \frac{ dr }{ d\theta } ( \theta ) = -r^2 \left( -b \sin \left( \theta + c \right) + 3 d \theta^2 + 4 e \theta^3 + 5 f \theta^4 + 6 g \theta^5 \right) \]
\pagebreak

\[ \frac{ d^2 r }{ d \theta^2 } ( \theta ) = 2 r^3 \left( -b \sin \left( \theta + c \right) + 3 d \theta^2 + 4 e \theta^3 + 5 f \theta^4 + 6 g \theta^5 \right)^2 - r^2 \left( -b \cos \left( \theta + c \right) + 6 d \theta + 12 e \theta^2 + 20 f \theta^3 + 30 g \theta^4 \right) \]
\pagebreak

\[ \frac{ d^2 r }{ d \theta^2 } ( \theta ) = \frac{ 2 }{ r } r^{ \prime 2 } - r^2 \left( -b \cos \left( \theta + c \right) + 6 d \theta + 12 e \theta^2 + 20 f \theta^3 + 30 g \theta^4 \right) \]
\pagebreak

\[ \frac{ d^3 r }{ d \theta^3 } ( \theta ) = -6 r^4 \left( -b \sin \left( \theta + c \right) + 3 d \theta^2 + 4 e \theta^3 + 5 f \theta^4 + 6 g \theta^5 \right)^3 + 6 r^3 \left( -b \sin \left( \theta + c \right) + 3 d \theta^2 + 4 e \theta^3 + 5 f \theta^4 + 6 g \theta^5 \right) \left( -b \cos \left( \theta + c \right) + d \theta + 12 e \theta^2 + 20 f \theta^3 + 30 g \theta^4 \right) - r^2 \left( b \sin \left( \theta + c \right) + 6 d + 24 e \theta + 60 f \theta^2 + 120 g \theta^3 \right) \]
\pagebreak

\[ \frac{ d^3 r }{ d \theta^3 } ( \theta ) = \frac{ 6 r^{ \prime 3 } }{ r^2 } - \frac{ 6 r^{ \prime } }{ r } \left( \frac{ 2 r^{ \prime 2 } }{ r } - r^{ \prime \prime } \right) - r^2 \left( b \sin \left( \theta + c \right) + 6 d + 24 e \theta + 60 f \theta^2 + 120 g \theta^3 \right) \]
\pagebreak

$ s = \frac{ r_1 + r_2 + c }{ 2 } $
\pagebreak

$ c = \sqrt{ r_1^2 + r_2^2 - 2 * r_1 * r_2 \cos( \theta ) } $
\pagebreak

$ \theta > \pi $
\pagebreak

$ \theta < \pi $
\pagebreak

$ a_m = s / 2 $
\pagebreak

$ 0 = t_f - F( x ) $
\pagebreak

$ F( x ) $
\pagebreak

$ x $
\pagebreak

\[ \phi ( \theta ) = \left( b_0 + b_1 \theta \right) \cos \theta + \left( b_2 + b_3 \theta \right) sin \theta \]
\pagebreak

$ \phi $
\pagebreak

$ ( b_0 ,b_1, b_2, b_3) $
\pagebreak

\[ \frac{ d \phi }{ d \theta } ( \theta ) = \left( b_1 + b_2 + b_3 \theta \right) \cos \theta - \left( b_0 + b_1 \theta - b_3 \right) \sin \theta \]
\pagebreak

\[ \frac{ d^2 \phi }{ d \theta^2 } ( \theta ) = \left( - b_0 - b_1 \theta + 2 b_3 \right) \cos \theta - \left( 2 b_1 + b_2 + b_3 \theta \right) \sin \theta \]
\pagebreak

\[ \frac{ d^3 \phi }{ d \theta^3 } ( \theta ) = - \left( 3 b_1 + b_2 + b_3 \theta \right) \cos \theta - \left( b_0 + b_1 \theta - 3 b_3 \right) \sin \theta \]
\pagebreak

$ ( b_0 ,b_1, b_2, b_3 ) $
\pagebreak

$ b_0 $
\pagebreak

$ b_1 $
\pagebreak

$ b_2 $
\pagebreak

$ b_3 $
\pagebreak

\[ \boldsymbol{a}_{apparent} = -\boldsymbol{a}_B - \dot{\boldsymbol{\omega}} \times \boldsymbol{r}_{ni} - \boldsymbol{\omega} \times (\boldsymbol{\omega} \times \boldsymbol{r}_{ni}) - 2(\boldsymbol{\omega} \times \boldsymbol{v}_{ni}) \]
\pagebreak

$\boldsymbol{a}_B$
\pagebreak

$\boldsymbol{\omega}$
\pagebreak

$\boldsymbol{r}_{ni}$
\pagebreak

$\boldsymbol{v}_{ni}$
\pagebreak

\[ \boldsymbol{a}_{centripetal} = -\boldsymbol{\omega} \times (\boldsymbol{\omega} \times \boldsymbol{r}_{ni}) \]
\pagebreak

\[ \boldsymbol{a}_{Coriolis} = -2(\boldsymbol{\omega} \times \boldsymbol{v}_{ni}) \]
\pagebreak

\[ \boldsymbol{a}_{Euler} = - \dot{\boldsymbol{\omega}} \times \boldsymbol{r}_{ni} \]
\pagebreak

$\dot{\boldsymbol{\omega}}$
\pagebreak

$y=a*x+b$
\pagebreak

$a$
\pagebreak

\begin{eqnarray*} x &=& r\cos\theta\sin\phi \\ y &=& r\sin\theta\sin\phi \\ z &=& r\cos\phi \\ \end{eqnarray*}
\pagebreak

\begin{eqnarray*} r &=& \sqrt{ x^{ 2 } + y^{ 2 } + z^{ 2 } } \\ \theta &=& \arctan\frac{ y }{ x } \\ \phi &=& \arccos\frac{ z }{ r } \\ \end{eqnarray*}
\pagebreak

\begin{eqnarray*} x &=& r\cos \theta \\ y &=& r\sin \theta \\ z &=& z \\ \end{eqnarray*}
\pagebreak

\begin{eqnarray*} x &=& r\cos \theta \\ y &=& r\sin \theta \\ z &=& z \\ \dot{x} &=& V_r\cos{\theta} - V_{\theta}\sin{theta} \\ \dot{y} &=& V_r\sin{\theta} + V_{\theta}\cos{theta} \\ \dot{z} &=& V_z \end{eqnarray*}
\pagebreak

$ \pi $
\pagebreak

\begin{eqnarray*} r &=& \sqrt{x^2+y^2} \\ \theta &=& \arctan{\frac{y}{x}} \\ z &=& z \end{eqnarray*}
\pagebreak

$\pi$
\pagebreak

$ V_r $
\pagebreak

$ V_{\theta} $
\pagebreak

$ V_z $
\pagebreak

\begin{eqnarray*} r &=& \sqrt{x^2+y^2} \\ \theta &=& \arctan{\frac{y}{x}} \\ z &=& z \\ V_r = \dot{r} &=& \frac{x\dot{x}+y\dot{y}}{\sqrt{x^2+y^2}} \\ V_{\theta} = r\dot{\theta} &=& \frac{x\dot{y}-y\dot{x}}{\sqrt{x^2+y^2}} \\ V_z = \dot{z} \end{eqnarray*}
\pagebreak

\begin{eqnarray*} \frac{ \partial U }{ \partial x } & = & \frac{ x }{ \sqrt{ x^2 + y^2 +z^2 } } \frac{ \partial U }{ \partial r } - \frac{ x z }{ ( x^2 + y^2 +z^2 ) \sqrt{ x^2 + y^2 } } \frac{ \partial U }{ \partial \phi } - \frac{ y }{ x^2 + y^2 } \frac{ \partial U }{ \partial \lambda } \\ \frac{ \partial U }{ \partial y } & = & \frac{ y }{ \sqrt{ x^2 + y^2 +z^2 } } \frac{ \partial U }{ \partial r } - \frac{ y z }{ ( x^2 + y^2 +z^2 ) \sqrt{ x^2 + y^2 } } \frac{ \partial U }{ \partial \phi } + \frac{ x }{ x^2 + y^2 } \frac{ \partial U }{ \partial \lambda } \\ \frac{ \partial U }{ \partial z } & = & \frac{ z }{ \sqrt{ x^2 + y^2 +z^2 } } \frac{ \partial U }{ \partial r } + \frac{ \sqrt{ x^2 + y^2 } } { x^2 + y^2 +z^2 } \frac{ \partial U }{ \partial \phi } \end{eqnarray*}
\pagebreak

$ y $
\pagebreak

$ z $
\pagebreak

$ U $
\pagebreak

$ \lambda $
\pagebreak

\begin{eqnarray*} x &=& r * \cos \phi * \cos \theta\\ y &=& r * \cos \phi * \sin \theta\\ z &=& r * \sin \phi\\ CartesianVelocities = T_{cyl2cart}*T_{sph2cyl}*SphericalVelocities \end{eqnarray*}
\pagebreak

\begin{eqnarray*} T_{sph2cyl} = [ \cos\phi , 0.0 , -\sin \phi ; 0.0 , 1.0 , 0.0 ; \sin\phi , 0.0 , \cos\phi ]\\ T_{cyl2cart} = [ \cos\theta , -\sin\theta , 0.0 ; \sin\theta , \cos\theta , 0.0 ; 0.0 , 0.0 , 1.0 ]\\ \end{eqnarray*}
\pagebreak

\begin{eqnarray*} r &=& \sqrt{ x^{ 2 } + y^{ 2 } + z^{ 2 } } \\ \phi &=& \arcsin\frac{ z }{ r } \\ \theta &=& \arctan\frac{ y }{ x } \\ SphericalVelocities = T_{cyl2sph}*T_{cart2cyl}*CartesianVelocities \end{eqnarray*}
\pagebreak

\begin{eqnarray*} T_{cyl2sph} = [ \cos\phi , 0.0 , \sin \phi ; 0.0 , 1.0 , 0.0 ; -\sin\phi , 0.0 , \cos\phi ]\\ T_{cart2cyl} = [ \cos\theta , \sin\theta , 0.0 ; -\sin\theta , \cos\theta , 0.0 ; 0.0 , 0.0 , 1.0 ]\\ \end{eqnarray*}
\pagebreak

$ P _{ n, m }( u ) $
\pagebreak

$ u $
\pagebreak

\[ P _{ n, m } ( u ) = ( 1 - u ^ 2 ) ^ { m / 2 } \frac{ d ^ m }{ du ^ m } \left[ P_n ( u ) \right] \textrm{ for }n \geq 0, 0 \leq m \leq n \]
\pagebreak

$ P_{ n, m }( u ) $
\pagebreak

$ n \geq 0, m \geq n $
\pagebreak

\[ P _{ n, m } ( u ) = 0 \textrm{ for }n \geq 0, m \geq n \]
\pagebreak

$ \bar{ P }_{ n, m }( u ) $
\pagebreak

\[ \bar{ P }_{ n, m } ( u ) = \Pi_{ n, m } P_{ n, m } ( u ) \]
\pagebreak

\[ \Pi_{ n, m } = \sqrt{ \frac{ ( 2 - \delta_{ 0, m } ) ( 2 n + 1 ) ( n - m )! } { ( n + m )! } } \]
\pagebreak

\[ P _{ n, m } ( u ) = ( 1 - u ^ 2 ) ^ { m / 2 } \frac{ d ^ m }{ du ^ m } \left[ P_n ( u ) \right] \]
\pagebreak

\[ \frac{ \mathrm{ d } P_{ n, m } ( u ) }{ \mathrm{ d } u } = \frac{ \sqrt{ 1 - u ^ 2 } P_{ n, m + 1 }( u ) - m u P_{ n, m }( u ) }{ 1 - u ^ 2 } \]
\pagebreak

$ P_{ n, m } ( u ) $
\pagebreak

$ P_{ n, m + 1 } ( u ) $
\pagebreak

\[ \frac{ \mathrm{ d } \bar{ P }_{ n, m } ( u ) }{ \mathrm{ d } u } = \sqrt{ \frac{ ( n + m + 1 )( n - m ) }{ ( 1 + \delta_{ 0, m } ) ( 1 - u^2 ) } } \bar{ P }_{ n, m + 1 } - \frac{ m u }{ 1 - u^2 } \bar{ P }_{ n, m } \]
\pagebreak

$ P_{ n, m }(u) $
\pagebreak

\begin{eqnarray*} P_{ 0, 0 }( u ) = 1 \\ P_{ 1, 0 }( u ) = u \\ P_{ 1, 1 }( u ) = \sqrt{ 1 - u^2 } \end{eqnarray*}
\pagebreak

$ n = 1 $
\pagebreak

$ m = 1 $
\pagebreak

$ \bar{ P }_{ n, m }(u) $
\pagebreak

\begin{eqnarray*} \bar{ P }_{ 0, 0 }( u ) = 1 \\ \bar{ P }_{ 1, 0 }( u ) = \sqrt{ 3 } u \\ \bar{ P }_{ 1, 1 }( u ) = \sqrt{ 3 - 3 u^2 } \end{eqnarray*}
\pagebreak

\[ P_{ n, m }( u ) = ( 2 n - 1 ) P_{ 1, 1 }( u ) P_{ n - 1, m - 1 }( u ) \]
\pagebreak

\[ \bar{ P }_{ n, m }( u ) = \sqrt{ \frac{ 2 n - 1 }{ 6 n } } \bar{ P }_{ 1, 1 }( u ) \bar{ P }_{ n - 1, m - 1 }( u ) \]
\pagebreak

\[ P_{ n, m }( u ) = \frac{ ( 2 n - 1 ) u P_{ n - 1, m }( u ) - ( n + m - 1 ) P_{ n - 2, m }( u ) }{ n - m } \]
\pagebreak

\[ \bar{ P }_{ n, m }( u ) = \sqrt{ \frac{ ( 2 n - 1 )( 2 n + 1 ) }{ ( n - m ) ( n + m ) } } u \bar{ P }_{ n - 1, m }( u ) - \sqrt{ \frac{ ( 2 n + 1 )( n + m - 1 ) ( n - m - 1 ) } { ( n - m)( n + m )( 2 n - 3 ) } } \bar{ P }_{ n - 2, m }( u ) \]
\pagebreak

$\approx$
\pagebreak

\[ U = A \left( \frac{ R }{ r} \right) ^{ n + 1} P _{ n, m } ( \sin \phi ) \left[ C _{ n, m } \cos( m \lambda ) + S _{ n, m } \sin( \lambda ) \right] \]
\pagebreak

$ A $
\pagebreak

$ R $
\pagebreak

$ P _{ n, m }( \sin \phi ) $
\pagebreak

$ \sin \phi $
\pagebreak

$ C _{ n, m } $
\pagebreak

$ S _{ n, m } $
\pagebreak

\begin{eqnarray*} \frac{ \mathrm{ d } U }{ \mathrm{ d } r } = -\frac{ A }{ r } \left( \frac{ R }{ r } \right) ^{ n + 1 } ( n + 1 ) P_{ n, m }( \sin \phi )[ C_{ n, m } \cos( m \lambda ) + S_{ n,m } \sin( m \lambda ) ] \\ \frac{ \mathrm{ d } U }{ \mathrm{ d } \phi } = A \left( \frac{ R }{ r } \right)^{ n + 1 } \frac{ \mathrm{ d } [ P( \sin \phi ) ] }{ \mathrm{ d } [ \sin \phi ] } \cos \phi [ C_{ n, m } \cos( m \lambda ) + S_{ n, m } \sin( m \lambda ) ] \\ \frac{ \mathrm{ d } U }{ \mathrm{ d } \lambda } = A \left( \frac{ R }{ r } \right)^{ n + 1 } m P_{ n, m }( \sin \phi ) [ S_{ n, m } \cos( m \lambda ) - C_{ n, m } \sin( m \lambda ) ] \end{eqnarray*}
\pagebreak

$ \alpha $
\pagebreak

$ \kappa $
\pagebreak

$ \beta $
\pagebreak

$ \gamma $
\pagebreak

$ \sqrt{ L + \lambda } $
\pagebreak

$ L $
\pagebreak

\[ \frac{ d^{ 3 } ( x, y, z ) } { du * dv^{ 2 } } \]
\pagebreak

\[ y_{target} = x_{1} * ( 1 - mu ) + x_{2} * mu \]
\pagebreak

$ mu = \frac{ x_{target} - x_{1} } { x_{2} + x_{1} } $
\pagebreak

$ x_{2} > x_{1} $
\pagebreak

$ \mu = \frac{ x_{target} - x_{1} } { x_{2} + x_{1} } $
\pagebreak

$f''(x_i)$
\pagebreak

$f(x_i)$
\pagebreak

$f'(x_i)$
\pagebreak

\[ x_{n+1} = x_n-\frac{2 F\left(x_n\right) F'\left(x_n\right)} {2 F'\left(x_n\right){}^2-F\left(x_n\right) F''\left(x_n\right)} \]
\pagebreak

\[ x_{n+1} = x_n - \frac{F\left(x_n\right)}{F'\left(x_n\right)} \]
\pagebreak

\[ x_{n+1} = x_n - F\left(x_n\right) \frac{\left(x_n - x_{n-1}\right)} {F\left(x_n\right) - F\left(x_{n-1}\right)} \]
\pagebreak

\[ \mu_{s} = \frac{ \sum_{i=1}^{N} X_{i} } { N } \]
\pagebreak

$\mu_{s}$
\pagebreak

$ N $
\pagebreak

$ X $
\pagebreak

\[ s^{2}_{s} = \frac{ 1 }{ N - 1 } * \sum_{i=1}^{N} X_{i} ( X_{i} - \bar{ X } )^{ 2 } ) \]
\pagebreak

$ s^{2}_{s} $
\pagebreak

$ \bar{ X } $
\pagebreak

\[ y = a + b * x \]
\pagebreak

$ b $
\pagebreak

$ a $
\pagebreak

\end{document}
